CoqOfRust/Proofs/M.v
@@ -79,3 +79,11 @@ Module Run.
   | Cast {A : Set} (state : State) (v : A) :
     t (LowM.Cast v) state v state.
 End Run.
+
+(** Simplify the usual case of read of immediate value. *)
+Lemma read_of_imm {A : Set} (v : A) :
+  M.read (Ref.Imm v) =
+  M.pure v.
+Proof.
+  reflexivity.
+Qed.
